implementation and correctness proof

Spec.CSwap.fst
@@ -1,28 +1,49 @@
 module Spec.CSwap
 
-(* Swapping two variables *)
+open FStar.UInt32
+let uint32 =  FStar.UInt32.t
 
-val cswap: x: nat -> y: nat -> c: nat{c = 0 \/ c = 1} -> Tot (nat * nat)
+(* Swapping two uint32 variables *)
+
+val cswap: x:uint32 -> y:uint32 -> c:uint32 ->
+  Tot (uint32 * uint32)
 let cswap x y c =
-  if c = 0 then
+  if c = 0ul then
     (x, y)
   else
     (y, x)
 
+val cswap_is_correct: x:uint32 -> y:uint32 -> c:uint32{c = 1ul \/ c = 0ul} -> Lemma
+  (ensures (
+    let a, b = cswap x y c in
+    if c = 0ul then
+      a = x /\ b = y
+    else
+      a = y /\ b = x
+  ))
+let cswap_is_correct x y c = ()
+
 (* Tests *)
 let test () =
-  let a = 123456789 in
-  let b = 9876543210 in
+  let a = 123456789ul in
+  let b = 987654321ul in
 
   (* Don't swap *)
-  let c, d = cswap a b 0 in
+  let c, d = cswap a b 0ul in
   if c = a && d = b then
     IO.print_string "SUCCESS\n"
   else
     IO.print_string "ERROR :/\n";
 
   (* Swap *)
-  let e, f = cswap a b 1 in
+  let e, f = cswap a b 1ul in
+  if e = b && f = a then
+    IO.print_string "SUCCESS\n"
+  else
+    IO.print_string "ERROR :/\n";
+
+  (* Swap *)
+  let e, f = cswap a b 0xFFFFFFFFul in
   if e = b && f = a then
     IO.print_string "SUCCESS\n"
   else
