Impl.CSwap.fst
@@ -1,0 +1,98 @@
+module Impl.CSwap
+
+open FStar.UInt32
+open FStar.UInt
+let uint32 = FStar.UInt32.t
+
+open Spec.CSwap
+
+(* Lemmata that help proving correctness. (A little more than necessary :) *)
+
+val xor_rules: a:uint32 -> b:uint32 -> c:uint32 -> Lemma
+  (ensures (UInt32.logxor a (UInt32.logxor a b) = b /\
+            UInt32.logxor a (UInt32.logxor b a) = b /\
+            UInt32.logxor a 0ul = a /\
+            UInt32.logxor a 0xFFFFFFFFul = UInt32.lognot a /\
+            UInt32.logxor (UInt32.logxor a b) c = UInt32.logxor a (UInt32.logxor b c)
+  ))
+let xor_rules x y z =
+  UInt.logxor_associative (v x) (v y) (v z);
+  UInt.logxor_associative (v x) (v x) (v y);
+  UInt.logxor_commutative (v x) (v y);
+  UInt.logxor_commutative (v 0ul) (v y);
+  UInt.logxor_self (v x);
+  UInt.logxor_lemma_1 (v x);
+  UInt.logxor_lemma_1 (v y);
+  UInt.logxor_lemma_2 (v x);
+  UInt.logxor_lemma_2 (v y)
+
+val and_rules: a:uint32 -> b:uint32{b = 0xFFFFFFFFul \/ b = 0ul} -> Lemma
+  (ensures (
+    UInt32.logand 0xFFFFFFFFul a = a /\
+    UInt32.logand 0ul a = 0ul /\
+    UInt32.logand a b = UInt32.logand b a /\
+    (if b = 0xFFFFFFFFul then UInt32.logand a b = a else UInt32.logand a b = 0ul)
+  ))
+let and_rules x y =
+  UInt.logand_lemma_1 (v x);
+  UInt.logand_lemma_2 (v x);
+  UInt.logand_commutative (v x) (v 0ul);
+  UInt.logand_commutative (v x) (v 0xFFFFFFFFul);
+  UInt.logand_commutative (v x) (v y)
+
+val cswap_step_rules: x:uint32 -> y:uint32 -> c:uint32{c = 0xFFFFFFFFul \/ c = 0ul} -> Lemma
+  (ensures (
+    let r = (x ^^ y) &^ c in
+    if c = 0xFFFFFFFFul then
+      r = x ^^ y
+    else
+      r = 0ul
+  ))
+let cswap_step_rules x y c =
+  xor_rules x y c;
+  and_rules (x ^^ y) c
+
+(* Swapping two uint32 variables in constant time *)
+
+val cswap_constant_time: x:uint32 -> y:uint32 -> c:uint32{c = 0xFFFFFFFFul \/ c = 0ul} ->
+  Tot (uint32 * uint32)
+let cswap_constant_time x y c =
+  let mask = (x ^^ y) &^ c in
+  let a = x ^^ mask in
+  let b = y ^^ mask in
+  (a, b)
+
+(* Prove correctness of the constant time conditional swap using Spec.CSwap. *)
+
+val cswap_constant_time_is_correct:
+  x:uint32 -> y:uint32 -> c:uint32{c = 0xFFFFFFFFul \/ c = 0ul} -> Lemma
+  (requires (
+    x = y /\ c = 0ul
+  ))
+  (ensures (
+    let a, b = cswap_constant_time x y c in
+    let c, d = cswap x y c in
+    a = c /\ b = d
+  ))
+let cswap_constant_time_is_correct x y c =
+  cswap_step_rules x y c;
+  xor_rules y x c
+
+(* Tests *)
+let test () =
+  let a = 123456789ul in
+  let b = 987654321ul in
+
+  (* Don't swap *)
+  let c, d = cswap_constant_time a b 0ul in
+  if c = a && d = b then
+    IO.print_string "SUCCESS\n"
+  else
+    IO.print_string "ERROR :/\n";
+
+  (* Swap *)
+  let e, f = cswap_constant_time a b 0xFFFFFFFFul in
+  if e = b && f = a then
+    IO.print_string "SUCCESS\n"
+  else
+    IO.print_string "ERROR :/\n"
