Makefile
@@ -1,4 +1,6 @@
 
+all: cswap.exe cswap_impl.exe
+
 cswap.exe: Spec.CSwap.fst
 	mkdir -p cswap-ml
 	fstar.exe --codegen OCaml --extract_module Spec.CSwap --odir cswap-ml $^
@@ -7,5 +9,13 @@ cswap.exe: Spec.CSwap.fst
 	OCAMLPATH="${PATH}" ocamlfind opt -package fstarlib -linkpkg -w -20-26-3-8-58 -w -8-20-26-28-10 -I cswap-ml cswap-ml/Spec_CSwap.ml -o cswap.exe
 	./cswap.exe
 
+cswap_impl.exe: Impl.CSwap.fst
+	mkdir -p cswap-ml
+	fstar.exe --z3rlimit 50 --codegen OCaml --extract_module Impl.CSwap --odir cswap-ml $^
+	@echo '\n\nlet _ = test()' >> cswap-ml/Impl_CSwap.ml
+	# This assumes that FStar/bin is in the PATH.
+	OCAMLPATH="${PATH}" ocamlfind opt -package fstarlib -linkpkg -w -20-26-3-8-58 -w -8-20-26-28-10 -I cswap-ml cswap-ml/Impl_CSwap.ml -o cswap_ct.exe
+	./cswap_ct.exe
+
 clean:
-	rm -rf cswap-ml cswap.exe
+	rm -rf cswap-ml cswap.exe cswap_ct.exe
